\documentclass{homework}

\usepackage{mathpazo}

\title{Homework 7}

\begin{document}

\maketitle

\begin{problem}{1}
%%%% %%%% %%%% %%%% %%%% %%%% %%%% %%%% %%%% %%%% %%%% %%%% %%%% %%%% %%%% %%%%|
Note that $\mathcal{D}_N$ can be divided into four cases:
\begin{itemize}
\item $0 \leq x, y < 1$.
      $A_N = \{(i, j) \in \mathcal{D}_N | 0 \leq i/2^N, j/2^N < 1\}$.
\item The top line of the square.
      $T_N = \{(i, 2^N) \in \mathcal{D}_N\}$.

\item The right line of the square.
      $R_N = \{(2^N, j) \in \mathcal{D}_N\}$.

\item All the rest, on which $f$ is always $0$.
\end{itemize}
Then, the upper sum and lower sum can be written as:
\begin{align*}
U_N(f) &= \sum_{C \in A_N} M_C(f) \mathrm{vol}_n C \\
       &+ \sum_{C \in T_N} M_C(f) \mathrm{vol}_n C \\
       &+ \sum_{C \in R_N} M_C(f) \mathrm{vol}_n C \\
       &= \sum_{(i, j) \in A_N}
          \sin(\frac{i - j}{2^N} + \frac{1}{2^N}) \frac{1}{2^{2N}}
        + 0 \\
       &+ \sum_{(i, j) \in R_N}
          \sin(1 - \frac{j}{2^N}) \frac{1}{2^{2N}}
\end{align*}
\begin{align*}
L_N(f) &= \sum_{C \in A_N} m_C(f) \mathrm{vol}_n C \\
       &= \sum_{(i, j) \in A_N}
          \sin(\frac{i - j}{2^N} - \frac{1}{2^N}) \frac{1}{2^{2N}} \\
\end{align*}
%%%% %%%% %%%% %%%% %%%% %%%% %%%% %%%% %%%% %%%% %%%% %%%% %%%% %%%% %%%% %%%%|
\begin{align*}
U_N(f) - L_N(f)
&= \sum_{(i, j)\in A_N}\sin(\frac{i-j}{2^N}+\frac{1}{2^N})\frac{1}{2^{2N}}
 - \sum_{(i, j)\in A_N}\sin(\frac{i-j}{2^N}-\frac{1}{2^N})\frac{1}{2^{2N}} \\
&+ \sum_{(i, j) \in R_N} \sin(1 - \frac{j}{2^N}) \frac{1}{2^{2N}} \\
&= \frac{1}{2^{2N}} \sum_{(i, j)\in A_N}
   2\cos(\frac{i-j}{2^N})\sin(\frac{1}{2^N})
 + \sum_{(i, j) \in R_N} \sin(1 - \frac{j}{2^N}) \frac{1}{2^{2N}} \\
&\leq \frac{1}{2^{2N}} \sum_{(i, j)\in A_N}
      2\cos(\frac{i-j}{2^N})\sin(\frac{1}{2^N})
    + \frac{1}{2^N} \cdot 1 \cdot \frac{1}{2^{2N}}
\end{align*}
Also, note that
$$\frac{1}{2^{2N}} \sum_{(i, j)\in A_N}
  2\cos(\frac{i-j}{2^N})\sin(\frac{1}{2^N})
  \leq U_N(f) - L_N(f)
$$
. Since $\sin(\frac{1}{2^N})$ goes to $0$ as $N$ goes to infinity, we have
$$\lim_{N \to \infty}
  \frac{1}{2^{2N}} \sum_{(i, j)\in A_N}
  2\cos(\frac{i-j}{2^N})\sin(\frac{1}{2^N})
  = 0
$$
. Moreover,
$$\lim_{N \to \infty} \frac{1}{2^N} = 0$$
. Therefore, by squeeze theorem,
$$\lim_{N \to \infty} U_N(f) - L_N(f) = 0$$
\QED
\end{problem}

\begin{problem}{2}
%%%% %%%% %%%% %%%% %%%% %%%% %%%% %%%% %%%% %%%% %%%% %%%% %%%% %%%% %%%% %%%%|
\textbf{Claim}.
Let $\epsilon > 0$, there exists $N_0$ such that for all $N > N_0$,
$U_N(f) - L_N(f) < \epsilon$.

Since $f$ is uniformly continuous, there exists $\delta$ such that
if $|\bpnt{x} - \bpnt{y}| \leq \delta$, then
$|f(\bpnt{x}) - f(\bpnt{y})| < \epsilon / \mathrm{vol}(\mathrm{Supp}(f))$.
Claim that $N_0$ is the smallest integer such that $1 / 2^{N_0 + 1} < \delta$.
Fix $\delta$.

Let $N > N_0$. Let $C \in \mathcal{D}_N$. Let $\bpnt{x}$ be the point of $C$
such that $f(\bpnt{x}) = M_C(f)$. For each $\bpnt{y} \in C$,
$$|\bpnt{x} - \bpnt{y}| \leq \frac{\sqrt{2}}{2^{N+1}}
< \frac{1}{2^{N_0+1}} < \delta$$
$$   M_C(f) - m_C(f)
\leq |f(\bpnt{x} - \bpnt{y}|
<\frac{\epsilon}{\mathrm{vol}(\mathrm{Supp}(f))}$$
Then,
\begin{align*}
U_N(f) - L_N(f)
&= \sum_{C \in \mathcal{D}_N} [M_C(f) - m_C(f)]\mathrm{vol}_n C\\
&< \sum_{C \in \mathcal{D}_N} \frac{\epsilon}{\mathrm{vol}(\mathrm{Supp}(f))}
    \mathrm{vol}_n C\\
&= \mathrm{vol}(\mathrm{Supp}(f))
    \frac{\epsilon}{\mathrm{vol}(\mathrm{Supp}(f))}\\
&= \epsilon
\end{align*}
. Clearly, $f$ is integrable. \QED
\end{problem}

\begin{problem}{3}
Let $R = \{(x, y) \in \mathbb{R}^2 | 0 \leq y \leq x \leq \pi\}$,
\begin{align*}
\int_0^\pi(\int_y^\pi \frac{\sin x}{x} \mathrm{d}x)\mathrm{d}y
&= \int_R \frac{\sin x}{x} |\mathrm{d} x \mathrm{d} y| \\
&= \int_0^{\pi} (\int_0^x \frac{\sin x}{x} \mathrm{d}y) \mathrm{d}x \\
&= \int_0^{\pi} \sin x \mathrm{d}x \\
&= - \cos \pi + \cos 0  = 2
\end{align*}
\end{problem}

\begin{problem}{4}
Let $R = \{(x, y) \in \mathbb{R}^2 | 0 \leq x \leq a, x^2 \leq y \leq a^2\}$,
\begin{align*}
\int_0^a (\int_{x^2}^{a^2} \sqrt{y}e^{-y^2} \mathrm{d}y) \mathrm{d}x
&= \int_R \sqrt{y}e^{-y^2} |\mathrm{d}x \mathrm{d}y| \\
&= \int_0^{a^2} (\int_{0}^{\sqrt{y}} \sqrt{y}e^{-y^2} \mathrm{d}x) \mathrm{d}y \\
&= \int_0^{a^2} ye^{-y^2} \mathrm{d}y \\
&= -\frac{1}{2}e^{-y^2} |_0^{a^2} \\
&= -\frac{1}{2}e^{-a^2} + \frac{1}{2}
\end{align*}
\end{problem}

\end{document}
